Add bakery spec

examples/Messaging/Bakery.v
@@ -3,7 +3,7 @@ From ITree Require Import
      CategoryOps
      Indexed.Sum.
 
-From Coq Require Import Nat List.
+From Coq Require Import Nat List Vector.
 
 From ExtLib Require Import
      Data.Nat
@@ -17,10 +17,12 @@ From CTree Require Import
      CTree
      Eq
      Interp.Network
+     Interp.Preempt
      Logic.Kripke
      Logic.Ctl.
 
-Import MonadNotation CtlNotations.
+Import MonadNotation CtlNotations ListNotations VectorNotations.
+Local Open Scope ctl_scope.
 Local Open Scope list_scope.
 Local Open Scope monad_scope.
 Local Open Scope ctree_scope.
@@ -35,23 +37,28 @@ Definition enter_cs {E C} `{csE -< E}: ctree E C unit :=
 Definition exit_cs {E C} `{csE -< E}: ctree E C unit :=
   trigger (In_CS false). 
 
-#[global] Instance handler_cs: csE ~~> state bool :=
+#[global] Instance handler_csE: csE ~~> state bool :=
   fun _ e => match e with
           | In_CS b => put b
           end.
 
 From CTree Require Import FoldStateT.
 
+(* A finite map of [uid] to their number *)
+Notation baker_map := (alist uid nat) (only parsing).
+
+Notation Client := (ctree ((netE uid +' parE) +' csE +' stateE (nat * baker_map)) B01 unit) (only parsing).
+
 (*| Client process |*)
-Definition client (id: uid)(bakery: uid): ctree (netE uid +' csE) B1 unit :=
+Definition client (baker: uid)(id: uid): Client :=
   CTree.forever (fun _ =>
       (* 1. Ask for a ticket number *)
-      send bakery id;;
+      send baker id;;
       (* 2. Loop until received [CS] message *)
       CTree.iter (fun _ =>
                     m <- recv;;
                     match m with
-                    | Some x => if x =? bakery then 
+                    | Some x => if x =? baker then 
                                  enter_cs;;
                                  (* DO WORK HERE*)
                                  exit_cs;;
@@ -61,9 +68,6 @@ Definition client (id: uid)(bakery: uid): ctree (netE uid +' csE) B1 unit :=
                     | None => Ret (inl tt)
                     end) tt) tt.
 
-(* A finite map of [uid] to their number *)
-Notation baker_map := (alist uid nat) (only parsing).
-
 (* Find the minimum number *)
 Definition alist_minv: baker_map -> option (uid * nat) :=
   fold_alist (fun k v acc => match acc with
@@ -72,10 +76,11 @@ Definition alist_minv: baker_map -> option (uid * nat) :=
                           end) None.
 
 (*| The baker process, synchronized access to CS through ticket |*)
-Definition baker(bkid: uid): ctree (netE uid +' stateE (nat * baker_map)) B1 unit :=
+Definition baker(bkid: uid): Client :=
   CTree.forever (fun _ =>
       (* 1. Schedule a Critical Section (CS) if possible *)
       '(cnt, book) <- get ;;
+      (* 1.1. Pick the user with smallest ID, if exists *)
       match alist_minv book with
       | None => Ret tt
       | Some (i, _) =>
@@ -84,7 +89,7 @@ Definition baker(bkid: uid): ctree (netE uid +' stateE (nat * baker_map)) B1 uni
           (* Baker sends his own [bkid] for client [i] to enter CS *)
           send i bkid 
       end ;;
-      (* 2. Listen to issue new ticket number *)
+      (* 2. Block to listen a new ticket number *)
       CTree.iter (fun _: unit =>
                     m <- recv;;
                     match m with
@@ -94,3 +99,30 @@ Definition baker(bkid: uid): ctree (netE uid +' stateE (nat * baker_map)) B1 uni
                     | None =>
                         Ret (inl tt)
                     end) tt) tt.
+
+Fixpoint range{A} n (f: nat -> A): vec n A :=
+  match n with
+  | 0 => []%vector
+  | S n' => (f n' :: range n' f)%vector
+  end.
+
+Notation requested_ticket bid i ts :=
+  <( now {(fun '(qs, _, _, _, _) => nth_error qs bid = Some (ts ++ [i]))})>.
+
+Notation entered_cs i :=
+  <( now {(fun '(_, id, cs, _, _) => cs = true /\ i = id)} )>.
+
+Check (rr (baker 0 :: range 3 (client 0))%vector).
+
+Definition init_state : (list (list uid) * uid * bool * uid * alist uid uid) :=
+  (List.nil, 0, false, 0, []%list).
+
+Lemma bakery_live: forall n i ts,
+    <( {rr (baker 0 :: range n (client 0))%vector},
+       init_state |= AG ({requested_ticket 0 i ts} -> AF {entered_cs i}))>.
+Proof.
+  intros.  
+  next.
+  split.
+  - intro H.
+Admitted.  
